WIP

src/lang/Memory.v
@@ -1,7 +1,9 @@
 Require Import Omega.
 
 Require Import sflib.
+Require Import paco.
 
+Require Import Axioms.
 Require Import Basic.
 Require Import DataStructure.
 Require Import Event.
@@ -9,7 +11,8 @@ Require Import Time.
 
 Set Implicit Arguments.
 
-Module Timestamps.
+
+Module Times.
   Definition t := LocFun.t Time.t.
   Definition init: t := LocFun.init Time.elt.
 
@@ -18,139 +21,340 @@ Module Timestamps.
 
   Definition get (loc:Loc.t) (c:t) :=
     LocFun.find loc c.
-End Timestamps.
+End Times.
 
-Module Commit.
+Module Snapshot.
   Structure t := mk {
-    reads: Timestamps.t;
-    writes: Timestamps.t;
+    reads: Times.t;
+    writes: Times.t;
   }.
 
-  Definition init: t := mk Timestamps.init Timestamps.init.
+  Definition init: t := mk Times.init Times.init.
 
   Inductive le (lhs rhs:t): Prop :=
   | le_intro
-      (READS: Timestamps.le lhs.(reads) rhs.(reads))
-      (WRITES: Timestamps.le lhs.(writes) rhs.(writes))
+      (READS: Times.le lhs.(reads) rhs.(reads))
+      (WRITES: Times.le lhs.(writes) rhs.(writes))
   .
 
   Inductive readable (history:t) (loc:Loc.t) (ts:Time.t): Prop :=
   | readable_intro
-      (* (CoRR: Time.le (Timestamps.get loc history.(Commit.reads)) ts) *)
-      (CoWR: Time.le (Timestamps.get loc history.(Commit.writes)) ts)
+      (* (CoRR: Time.le (Times.get loc history.(Snapshot.reads)) ts) *)
+      (CoWR: Time.le (Times.get loc history.(Snapshot.writes)) ts)
   .
 
   Inductive writable (history:t) (loc:Loc.t) (ts:Time.t): Prop :=
   | writable_intro
-      (CoRW: Time.lt (Timestamps.get loc history.(Commit.reads)) ts)
-      (CoWW: Time.lt (Timestamps.get loc history.(Commit.writes)) ts)
+      (CoRW: Time.lt (Times.get loc history.(Snapshot.reads)) ts)
+      (CoWW: Time.lt (Times.get loc history.(Snapshot.writes)) ts)
   .
-End Commit.
-
-
-Module ThreadCommit.
-  Structure t := mk {
-    current: Commit.t;
-    released: LocFun.t Commit.t;
-    acquirable: Commit.t;
-  }.
-
-  Definition init: t := mk Commit.init (LocFun.init Commit.init) Commit.init.
-
-  Inductive le (lhs rhs:t): Prop :=
-  | le_intro
-      (CURRENT: Commit.le lhs.(current) rhs.(current))
-      (RELEASED: forall (loc:Loc.t), Commit.le (LocFun.find loc lhs.(released)) (LocFun.find loc rhs.(released)))
-      (ACQUIRABLE: Commit.le lhs.(acquirable) rhs.(acquirable))
-  .
-
-  Inductive read
-            (tc1:t) (loc:Loc.t) (ts:Time.t) (released:Commit.t) (ord:Ordering.t)
-            (tc2:t): Prop :=
-  | read_intro
-      (FUTURE: le tc1 tc2)
-      (READABLE: Commit.readable tc1.(current) loc ts)
-      (READ: Time.le ts (Timestamps.get loc tc2.(current).(Commit.reads)))
-      (ACQUIRE: forall (ORDERING: Ordering.le Ordering.acquire ord),
-          Commit.le released tc2.(current))
-      (ACQUIRABLE: Commit.le released tc2.(acquirable))
-  .
-
-  Inductive write
-            (tc1:t) (loc:Loc.t) (ts:Time.t) (released:Commit.t) (ord:Ordering.t)
-            (tc2:t): Prop :=
-  | write_intro
-      (FUTURE: le tc1 tc2)
-      (WRITABLE: Commit.writable tc1.(current) loc ts)
-      (WRITE: Time.le ts (Timestamps.get loc tc2.(current).(Commit.writes)))
-      (RELEASE: forall (ORDERING: Ordering.le Ordering.release ord),
-          Commit.le tc2.(current) released)
-      (RELEASED: Commit.le (LocFun.find loc tc2.(ThreadCommit.released)) released)
-  .
-
-  Inductive fence
-            (tc1:t) (ord:Ordering.t)
-            (tc2:t): Prop :=
-  | fence_intro
-      (FUTURE: le tc1 tc2)
-      (ACQUIRE: forall (ORDERING: Ordering.le Ordering.acquire ord),
-          Commit.le tc2.(acquirable) tc2.(current))
-      (RELEASE: forall (ORDERING: Ordering.le Ordering.release ord) loc,
-          Commit.le tc2.(current) (LocFun.find loc tc2.(released)))
-  .
-End ThreadCommit.
-
-Module ThreadLocal.
-  Structure t := mk {
-    tc: ThreadCommit.t;
-    declares: IntervalSets.t;
-  }.
-
-  Definition init := mk ThreadCommit.init IntervalSets.bot.
-
-  Inductive declare
-            (loc:Loc.t) (ts0 ts:Time.t)
-            (declares1:IntervalSets.t) (used1:IntervalSets.t):
-    forall (declares2:IntervalSets.t) (used2:IntervalSets.t), Prop :=
-  | declare_alloc
-      (DISJOINT: IntervalSets.disjoint loc ts0 ts used1):
-      declare loc ts0 ts declares1 used1
-              (IntervalSets.add loc ts0 ts declares1)
-              (IntervalSets.add loc ts0 ts used1)
-  | declare_split
-      ts1 declares2
-      (MEM: IntervalSets.remove loc ts0 ts1 declares1 = Some declares2):
-      declare loc ts0 ts declares1 used1
-              (IntervalSets.add loc ts0 ts (IntervalSets.add loc ts ts1 declares2))
-              used1
-  .
-End ThreadLocal.
-
+End Snapshot.
 
 Module Message.
   Structure t := mk {
     val: Const.t;
-    released: Commit.t;
+    released: Snapshot.t;
   }.
-
-  Inductive future: forall (lhs rhs:option t), Prop :=
-  | future_None rhs:
-      future None rhs
-  | future_Some msg:
-      future (Some msg) (Some msg)
-  .
+  Definition elt: t := mk 0 Snapshot.init.
 End Message.
 
-Module MessageSet.
-  Definition t := LocFun.t (TimeFun.t (option Message.t)).
-  Definition empty: t := LocFun.init (TimeFun.init None).
+Module Cell.
+  Structure t := mk {
+    messages: Time.t -> (option (Time.t * Message.t));
 
-  Definition get (loc:Loc.t) (ts:Time.t) (m:t): option Message.t :=
-    TimeFun.find ts (LocFun.find loc m).
+    VOLUME:
+      forall to from msg
+        (MESSAGE: messages to = Some (from, msg)),
+        Time.lt from to;
+  }.
 
-  Definition set (loc:Loc.t) (ts:Time.t) (msg:Message.t) (m:t): t :=
-    LocFun.add loc (TimeFun.add ts (Some msg) (LocFun.find loc m)) m.
-End MessageSet.
+  Definition wf (cell:t): Prop :=
+    forall to1 to2 from1 from2 msg1 msg2
+      (TO: to1 <> to2)
+      (MESSAGE1: cell.(messages) to1 = Some (from1, msg1))
+      (MESSAGE2: cell.(messages) to2 = Some (from2, msg2)),
+      Interval.disjoint (from1, to1) (from2, to2).
+
+  Lemma extensionality lhs rhs
+        (MESSAGES: forall x, lhs.(messages) x = rhs.(messages) x):
+    lhs = rhs.
+  Proof.
+    destruct lhs, rhs.
+    cut (messages0 = messages1).
+    { i. subst. f_equal. apply proof_irrelevance. }
+    extensionality to. auto.
+  Qed.
+
+  Definition le (lhs rhs:t): Prop :=
+    forall to from msg (MSG: lhs.(messages) to = Some (from, msg)),
+      rhs.(messages) to = Some (from, msg).
+
+  Program Definition init: t :=
+    mk
+      (TimeFun.add Time.elt (Some (Time.decr Time.elt, Message.mk 0 Snapshot.init)) (TimeFun.init None))
+      _.
+  Next Obligation.
+    unfold TimeFun.add in *.
+    match goal with
+    | [H: context[if ?c then _ else _] |- _] => destruct c
+    end;
+      inv MESSAGE.
+    apply Time.decr_spec.
+  Qed.
+
+  Lemma init_wf: wf init.
+  Proof.
+    unfold wf, init. i. simpl in *.
+    unfold TimeFun.add in *.
+    repeat
+      match goal with
+      | [H: context[if ?c then _ else _] |- _] => destruct c
+      | [H: Some _ = Some _ |- _] => inv H
+      end;
+      try inv MESSAGE1;
+      try inv MESSAGE2.
+    congruence.
+  Qed.
+
+  Inductive own (cell:t) (ts:Time.t): Prop :=
+  | own_intro
+      to from msg
+      (MESSAGE: cell.(messages) to = Some (from, msg))
+      (INTERVAL: Interval.mem (from, to) ts)
+  .
+
+  Definition disjoint (lhs rhs:t): Prop :=
+    forall ts (LHS: own lhs ts) (RHS: own rhs ts), False.
+
+  Lemma disjoint_comm lhs rhs
+        (DISJ: disjoint lhs rhs):
+    disjoint rhs lhs.
+  Proof.
+    ii. eapply DISJ; eauto.
+  Qed.
+
+  Lemma disjoint_messages
+        to lhs rhs lx rx
+        (DISJ: disjoint lhs rhs)
+        (LHS: lhs.(messages) to = Some lx)
+        (RHS: rhs.(messages) to = Some rx):
+    False.
+  Proof.
+    destruct lx, rx.
+    eapply DISJ; econs; eauto.
+    - apply Interval.mem_ub. eapply VOLUME. eauto.
+    - apply Interval.mem_ub. eapply VOLUME. eauto.
+  Qed.
+
+  Program Definition join (lhs rhs:t): t :=
+    mk
+      (fun x =>
+         match lhs.(messages) x, rhs.(messages) x with
+         | Some _, Some _ => Some (Time.decr x, Message.elt)
+         | Some lhs, None => Some lhs
+         | None, Some rhs => Some rhs
+         | None, None => None
+         end)
+      _.
+  Next Obligation.
+    destruct (messages lhs to) as [[]|] eqn:LHS,
+             (messages rhs to) as [[]|] eqn:RHS; try inv MESSAGE.
+    - apply Time.decr_spec.
+    - exploit (lhs.(VOLUME)); eauto.
+    - exploit (rhs.(VOLUME)); eauto.
+  Qed.
+
+  Lemma join_wf
+        lhs rhs
+        (DISJ: disjoint lhs rhs)
+        (LHS: wf lhs)
+        (RHS: wf rhs):
+    wf (join lhs rhs).
+  Proof.
+    ii. simpl in *.
+    destruct (messages lhs to1) as [[]|] eqn:LHS1,
+             (messages rhs to1) as [[]|] eqn:RHS1;
+      inv MESSAGE1;
+    destruct (messages lhs to2) as [[]|] eqn:LHS2,
+             (messages rhs to2) as [[]|] eqn:RHS2;
+      inv MESSAGE2;
+      try (eapply (disjoint_messages to1); eauto; fail);
+      try (eapply (disjoint_messages to2); eauto; fail).
+    - eapply LHS; eauto.
+    - eapply DISJ; econs; eauto.
+    - eapply DISJ; econs; eauto.
+    - eapply RHS; eauto.
+  Qed.
+
+  Lemma join_assoc x y z:
+    join (join x y) z = join x (join y z).
+  Proof.
+    apply extensionality. simpl. i.
+    destruct (messages x x0), (messages y x0), (messages z x0); auto.
+  Qed.
+
+  Lemma join_le
+        lhs rhs
+        (DISJ: disjoint lhs rhs):
+    le lhs (join lhs rhs).
+  Proof.
+    unfold join. ii. simpl in *.
+    destruct (messages lhs to) as [[]|] eqn:LHS,
+             (messages rhs to) as [[]|] eqn:RHS;
+      try congruence.
+    exfalso. eapply disjoint_messages; eauto.
+  Qed.
+
+  Lemma join_spec
+        lhs rhs b
+        (DISJ: disjoint lhs rhs)
+        (LHS: le lhs b)
+        (RHS: le rhs b):
+    le (join lhs rhs) b.
+  Proof.
+    unfold join. ii. simpl in *.
+    destruct (messages lhs to) as [[]|] eqn:LHS1,
+             (messages rhs to) as [[]|] eqn:RHS1;
+      inv MSG;
+      try congruence.
+    - exfalso. eapply disjoint_messages; eauto.
+    - apply LHS. auto.
+    - apply RHS. auto.
+  Qed.
+
+  Lemma join_comm lhs rhs:
+    join lhs rhs = join rhs lhs.
+  Proof.
+    apply extensionality. simpl. i.
+    destruct (messages lhs x), (messages rhs x); auto.
+  Qed.
+
+  Program Definition sub (lhs rhs:t): t :=
+    mk
+      (fun x =>
+         match lhs.(messages) x, rhs.(messages) x with
+         | _, Some _
+         | None, _ => None
+         | Some lhs, None => Some lhs
+         end)
+      _.
+  Next Obligation.
+    destruct (messages lhs to) eqn:LHS, (messages rhs to) eqn:RHS; inv MESSAGE.
+    eapply VOLUME; eauto.
+  Qed.
+
+  Lemma sub_wf
+        lhs rhs
+        (LHS: wf lhs)
+        (RHS: wf rhs):
+    wf (sub lhs rhs).
+  Proof.
+    ii. simpl in *.
+    destruct (messages lhs to1) as [[]|] eqn:LHS1,
+             (messages rhs to1) as [[]|] eqn:RHS1;
+      inv MESSAGE1;
+    destruct (messages lhs to2) as [[]|] eqn:LHS2,
+             (messages rhs to2) as [[]|] eqn:RHS2;
+      inv MESSAGE2;
+      try (eapply (disjoint_messages to1); eauto; fail);
+      try (eapply (disjoint_messages to2); eauto; fail).
+    eapply LHS; eauto.
+  Qed.
+
+  Lemma sub_le lhs rhs:
+    le (sub lhs rhs) lhs.
+  Proof.
+    unfold sub. ii. simpl in *.
+    destruct (messages lhs to) as [[]|] eqn:LHS,
+             (messages rhs to) as [[]|] eqn:RHS;
+      congruence.
+  Qed.
+
+  Lemma sub_spec lhs rhs
+        (DISJ: disjoint lhs rhs):
+    sub (join lhs rhs) rhs = lhs.
+  Proof.
+    apply extensionality. simpl. i.
+    destruct (messages lhs x) as [[]|] eqn:LHS,
+             (messages rhs x) as [[]|] eqn:RHS;
+      try congruence.
+    exfalso. eapply disjoint_messages; eauto.
+  Qed.
+End Cell.
+
+Module Memory.
+  Definition t := Loc.t -> Cell.t.
+  Definition wf (mem:t): Prop := forall loc, Cell.wf (mem loc).
+  Definition le (lhs rhs:t): Prop := forall loc, Cell.le (lhs loc) (rhs loc).
+
+  Definition init: t := LocFun.init Cell.init.
+  Lemma init_wf: wf init.
+  Proof. intro loc. apply Cell.init_wf. Qed.
+
+  Definition disjoint (lhs rhs:t): Prop :=
+    forall loc, Cell.disjoint (lhs loc) (rhs loc).
+
+  Lemma disjoint_comm lhs rhs
+        (DISJ: disjoint lhs rhs):
+    disjoint rhs lhs.
+  Proof.
+    intro loc. specialize (DISJ loc).
+    apply Cell.disjoint_comm. auto.
+  Qed.
+
+  Definition join (lhs rhs:t): t :=
+    fun loc => Cell.join (lhs loc) (rhs loc).
+
+  Lemma join_wf
+        lhs rhs
+        (DISJ: disjoint lhs rhs)
+        (LHS: wf lhs)
+        (RHS: wf rhs):
+    wf (join lhs rhs).
+  Proof. intro loc. apply Cell.join_wf; auto. Qed.
+
+  Lemma join_assoc x y z:
+    join (join x y) z = join x (join y z).
+  Proof. extensionality loc. apply Cell.join_assoc. Qed.
+
+  Lemma join_le
+        lhs rhs
+        (DISJ: disjoint lhs rhs):
+    le lhs (join lhs rhs).
+  Proof. intro loc. apply Cell.join_le; auto. Qed.
+
+  Lemma join_spec
+        lhs rhs b
+        (DISJ: disjoint lhs rhs)
+        (LHS: le lhs b)
+        (RHS: le rhs b):
+    le (join lhs rhs) b.
+  Proof. intro loc. apply Cell.join_spec; auto. Qed.
+
+  Lemma join_comm lhs rhs:
+    join lhs rhs = join rhs lhs.
+  Proof. extensionality loc. apply Cell.join_comm. Qed.
+
+  Definition sub (lhs rhs:t): t :=
+    fun loc => Cell.sub (lhs loc) (rhs loc).
+
+  Lemma sub_wf
+        lhs rhs
+        (LHS: wf lhs)
+        (RHS: wf rhs):
+    wf (sub lhs rhs).
+  Proof. intro loc. apply Cell.sub_wf; auto. Qed.
+
+  Lemma sub_le lhs rhs:
+    le (sub lhs rhs) lhs.
+  Proof. intro loc. apply Cell.sub_le. Qed.
+
+  Lemma sub_spec lhs rhs
+        (DISJ: disjoint lhs rhs):
+    sub (join lhs rhs) rhs = lhs.
+  Proof. extensionality loc. apply Cell.sub_spec. auto. Qed.
+End Memory.
+
 
 Module Memory.
   Structure t := mk {
@@ -163,7 +367,7 @@ Module Memory.
   Inductive step (thl1:ThreadLocal.t) (mem1:t): forall (e:option MemEvent.t) (thl2:ThreadLocal.t), Prop :=
   | step_read
       loc val ts released ord tc2
-      (READ: ThreadCommit.read thl1.(ThreadLocal.tc) loc ts released ord tc2)
+      (READ: Commit.read thl1.(ThreadLocal.tc) loc ts released ord tc2)
       (DECLARE: ~ IntervalSets.mem loc ts thl1.(ThreadLocal.declares))
       (MESSAGE: MessageSet.get loc ts mem1.(messages) = Some (Message.mk val released)):
       step thl1 mem1
@@ -171,7 +375,7 @@ Module Memory.
            (ThreadLocal.mk tc2 thl1.(ThreadLocal.declares))
   | step_write
       loc val ts0 ts released ord tc2 declares2
-      (WRITE: ThreadCommit.write thl1.(ThreadLocal.tc) loc ts released ord tc2)
+      (WRITE: Commit.write thl1.(ThreadLocal.tc) loc ts released ord tc2)
       (DECLARE: IntervalSets.remove loc ts0 ts thl1.(ThreadLocal.declares) = Some declares2)
       (MESSAGE: MessageSet.get loc ts mem1.(messages) = Some (Message.mk val released)):
       step thl1 mem1
@@ -179,9 +383,9 @@ Module Memory.
            (ThreadLocal.mk tc2 declares2)
   | step_update
       loc valr tsr releasedr valw tsw releasedw ord tc2 tc3 declares3
-      (READ: ThreadCommit.read thl1.(ThreadLocal.tc) loc tsr releasedr ord tc2)
-      (WRITE: ThreadCommit.write tc2 loc tsw releasedw ord tc3)
-      (RELEASE: Commit.le releasedr releasedw)
+      (READ: Commit.read thl1.(ThreadLocal.tc) loc tsr releasedr ord tc2)
+      (WRITE: Commit.write tc2 loc tsw releasedw ord tc3)
+      (RELEASE: Snapshot.le releasedr releasedw)
       (DECLARE: IntervalSets.remove loc tsr tsw thl1.(ThreadLocal.declares) = Some declares3)
       (MESSAGE1: MessageSet.get loc tsr mem1.(messages) = Some (Message.mk valr releasedr))
       (MESSAGE2: MessageSet.get loc tsw mem1.(messages) = Some (Message.mk valw releasedw)):
@@ -190,13 +394,13 @@ Module Memory.
            (ThreadLocal.mk tc3 declares3)
   | step_fence
       ord tc2
-      (FENCE: ThreadCommit.fence thl1.(ThreadLocal.tc) ord tc2):
+      (FENCE: Commit.fence thl1.(ThreadLocal.tc) ord tc2):
       step thl1 mem1
            (Some (MemEvent.fence ord))
            (ThreadLocal.mk tc2 thl1.(ThreadLocal.declares))
   | step_None
       tc2
-      (COMMIT: ThreadCommit.le thl1.(ThreadLocal.tc) tc2):
+      (COMMIT: Commit.le thl1.(ThreadLocal.tc) tc2):
       step thl1 mem1
            None
            (ThreadLocal.mk tc2 thl1.(ThreadLocal.declares))
@@ -204,23 +408,105 @@ Module Memory.
 
   Inductive declare (thl1:ThreadLocal.t) (mem1:t): forall (thl2:ThreadLocal.t) (mem2:t), Prop :=
   | declare_intro
-      loc ts val released ts0 tc2 declares2 used2
+      loc ts val released ts0 declares2 used2
       (TS: Time.lt ts0 ts)
-      (COMMIT: ThreadCommit.le thl1.(ThreadLocal.tc) tc2)
       (LOCAL: ThreadLocal.declare loc ts0 ts thl1.(ThreadLocal.declares) mem1.(used) declares2 used2)
       (GET: MessageSet.get loc ts mem1.(messages) = None):
       declare thl1 mem1
-              (ThreadLocal.mk tc2 declares2)
+              (ThreadLocal.mk thl1.(ThreadLocal.tc) declares2)
               (mk (MessageSet.set loc ts (Message.mk val released) mem1.(messages))
                   used2)
   .
 
+  (* TODO: messages are in rhs.(used)? *)
   Inductive future (declares:IntervalSets.t) (lhs rhs:t): Prop :=
   | future_intro
       (MESSAGE: forall loc ts, Message.future (MessageSet.get loc ts lhs.(messages)) (MessageSet.get loc ts rhs.(messages)))
-      (NONPERM:
-         forall loc ts (DECL: IntervalSets.mem loc ts declares),
+      (DECLARE:
+         forall loc ts (DECLARE: IntervalSets.mem loc ts declares),
            MessageSet.get loc ts lhs.(messages) = MessageSet.get loc ts rhs.(messages))
       (PERM: IntervalSets.le lhs.(used) rhs.(used))
   .
 End Memory.
+
+
+
+
+Module Commit.
+  Structure t := mk {
+    current: Snapshot.t;
+    released: LocFun.t Snapshot.t;
+    acquirable: Snapshot.t;
+  }.
+
+  Definition init: t := mk Snapshot.init (LocFun.init Snapshot.init) Snapshot.init.
+
+  Inductive le (lhs rhs:t): Prop :=
+  | le_intro
+      (CURRENT: Snapshot.le lhs.(current) rhs.(current))
+      (RELEASED: forall (loc:Loc.t), Snapshot.le (LocFun.find loc lhs.(released)) (LocFun.find loc rhs.(released)))
+      (ACQUIRABLE: Snapshot.le lhs.(acquirable) rhs.(acquirable))
+  .
+
+  Inductive read
+            (tc1:t) (loc:Loc.t) (ts:Time.t) (released:Snapshot.t) (ord:Ordering.t)
+            (tc2:t): Prop :=
+  | read_intro
+      (FUTURE: le tc1 tc2)
+      (READABLE: Snapshot.readable tc1.(current) loc ts)
+      (READ: Time.le ts (Times.get loc tc2.(current).(Snapshot.reads)))
+      (ACQUIRE: forall (ORDERING: Ordering.le Ordering.acquire ord),
+          Snapshot.le released tc2.(current))
+      (ACQUIRABLE: Snapshot.le released tc2.(acquirable))
+  .
+
+  Inductive write
+            (tc1:t) (loc:Loc.t) (ts:Time.t) (released:Snapshot.t) (ord:Ordering.t)
+            (tc2:t): Prop :=
+  | write_intro
+      (FUTURE: le tc1 tc2)
+      (WRITABLE: Snapshot.writable tc1.(current) loc ts)
+      (WRITE: Time.le ts (Times.get loc tc2.(current).(Snapshot.writes)))
+      (RELEASE: forall (ORDERING: Ordering.le Ordering.release ord),
+          Snapshot.le tc2.(current) released)
+      (RELEASED: Snapshot.le (LocFun.find loc tc2.(Commit.released)) released)
+  .
+
+  Inductive fence
+            (tc1:t) (ord:Ordering.t)
+            (tc2:t): Prop :=
+  | fence_intro
+      (FUTURE: le tc1 tc2)
+      (ACQUIRE: forall (ORDERING: Ordering.le Ordering.acquire ord),
+          Snapshot.le tc2.(acquirable) tc2.(current))
+      (RELEASE: forall (ORDERING: Ordering.le Ordering.release ord) loc,
+          Snapshot.le tc2.(current) (LocFun.find loc tc2.(released)))
+  .
+End Commit.
+
+Module ThreadLocal.
+  Structure t := mk {
+    tc: Commit.t;
+    declares: IntervalSets.t;
+  }.
+
+  Definition init := mk Commit.init IntervalSets.bot.
+
+  Inductive declare
+            (loc:Loc.t) (ts0 ts:Time.t)
+            (declares1:IntervalSets.t) (used1:IntervalSets.t):
+    forall (declares2:IntervalSets.t) (used2:IntervalSets.t), Prop :=
+  | declare_alloc
+      (DISJOINT: IntervalSets.disjoint loc ts0 ts used1):
+      declare loc ts0 ts declares1 used1
+              (IntervalSets.add loc ts0 ts declares1)
+              (IntervalSets.add loc ts0 ts used1)
+  | declare_split
+      ts1 declares2
+      (TIME: Time.lt ts ts1)
+      (DECLARE: IntervalSets.remove loc ts0 ts1 declares1 = Some declares2):
+      declare loc ts0 ts declares1 used1
+              (IntervalSets.add loc ts0 ts (IntervalSets.add loc ts ts1 declares2))
+              used1
+  .
+End ThreadLocal.
