src/lib/Axioms.v
@@ -1,0 +1,6 @@
+Require Export Classical.
+Require Export FunctionalExtensionality.
+
+Axiom prop_ext:
+  forall (P Q : Prop), 
+    (P <-> Q) -> P = Q.
